PrincInh/NFTerms.v
@@ -4,8 +4,6 @@ Require Import Autosubst.Autosubst.
 
 Require Import PrincInh.Utils.
 Require Import PrincInh.Terms.
-Require Import PrincInh.TypesCommon.
-Require Import PrincInh.TypesType.
 
 Import ListNotations.
 Import EqNotations.
@@ -83,52 +81,7 @@ Defined.
   
 Instance eqdec_nfterm : EqDec nfterm eq. unfold EqDec. apply eqdec_nfterm_fix. Defined.
 
-Inductive nfty (Gamma : repo) : nfterm -> type -> Type :=
-| NFTy_lam s sigma tau : nfty (sigma :: Gamma) s tau -> nfty Gamma (\__ s) (sigma ~> tau)
-| NFTy_var x tau ts ms : nth_error Gamma x = Some (make_arrow_type ts tau) ->             
-                         length ms = length ts ->
-                         (forall n (pms : n < length ms) (pts : n < length ts),
-                             nfty Gamma (nth_ok ms n pms) (nth_ok ts n pts)) ->
-             nfty Gamma (!!x @@ ms) tau
-.
 
-Inductive nfty_long (Gamma : repo) : nfterm -> type -> Type :=
-| NFTy_lam_long s sigma tau : nfty_long (sigma :: Gamma) s tau -> nfty_long Gamma (\__ s) (sigma ~> tau)
-| NFTy_var_long : forall x a ts ms (Gammaok : nth_error Gamma x = Some (make_arrow_type ts (? a)))
-                    (Lenproof : length ms = length ts),
-    (forall n (pms : n < length ms),
-        nfty_long Gamma (nth_ok ms n pms) (nth_ok ts n (rew Lenproof in pms))) ->
-    nfty_long Gamma (!!x @@ ms) (? a)
-.
-
-Inductive nfty_long_subj : forall Gamma Gamma' m m' rho rho', nfty_long Gamma m rho -> nfty_long Gamma' m' rho' -> Type :=
-| nfty_long_refl : forall Gamma m rho (proof: nfty_long Gamma m rho), nfty_long_subj _ _ _ _ _ _ proof proof
-| nfty_long_trans : forall Gamma Gamma' Gamma'' m m' m'' rho rho' rho''
-                      (proof1 : nfty_long Gamma m rho)
-                      (proof2 : nfty_long Gamma' m' rho')
-                      (proof3 : nfty_long Gamma'' m'' rho''),
-    nfty_long_subj _ _ _ _ _ _ proof1 proof2 ->
-    nfty_long_subj _ _ _ _ _ _ proof2 proof3 ->
-    nfty_long_subj _ _ _ _ _ _ proof1 proof3
-| nfty_long_subj_I : forall Gamma sigma tau s (proof : nfty_long (sigma :: Gamma) s tau),
-    nfty_long_subj _ _ _ _ _ _ proof (NFTy_lam_long _ _ _ _ proof)
-| nfty_long_subj_E : forall Gamma x ts ms a
-                       (Gammaok : nth_error Gamma x = Some (make_arrow_type ts (? a)))
-                       (Lenproof : length ms = length ts)
-                       (proofs : (forall n (pms : n < length ms),
-                                     nfty_long Gamma (nth_ok ms n pms) (nth_ok ts n (rew Lenproof in pms))))
-                       n (len: n < length ms),   
-    nfty_long_subj _ _ _ _ _ _ (proofs n len) (NFTy_var_long _ _ _ _ _ Gammaok Lenproof proofs).
-
-
-Lemma nfty_long_subterm : forall n m, subterm_nf n m -> forall tau Gamma, nfty_long Gamma m tau -> {Gamma' & {tau' & nfty_long Gamma' n tau'}}.
-Proof.
-  induction 1; intros.
-  - exists Gamma. exists tau. assumption.
-  - inv X0. eapply IHX. exact X1.
-  - inv X0. apply In_nth_error_set in i. destruct i as [n H].
-    apply nth_error_nth_ok in H. destruct H as [lp H]. pose proof (X1 n lp). eapply IHX. rewrite H in X0. exact X0.
-Qed.
 
 
 Fixpoint NFterm_term nft : term :=
